LList.v
@@ -1,0 +1,305 @@
+
+Set Implicit Arguments.
+
+Require Import List Eqdep_dec.
+
+Definition llist A n := {l : list A | length l = n}.
+
+Lemma ll_proj_eq A n : forall (l l' : llist A n), proj1_sig l = proj1_sig l' -> l = l'.
+ intros.
+ destruct l.
+ destruct l'.
+ simpl in H.
+ subst.
+ f_equal.
+ apply eq_proofs_unicity.
+ decide equality.
+Defined.
+
+  Import Plus.
+
+
+Program Definition llrev A n (l : llist A n) : llist A n := 
+  rev l.
+Obligation 1.
+ destruct l.
+ revert n e.
+ induction x; intros.
+  simpl in *; subst; reflexivity.
+  simpl in *; subst.
+  rewrite app_length.
+  simpl.
+  rewrite (IHx (length x)) by reflexivity.
+  rewrite <- plus_Snm_nSm.
+  rewrite plus_0_r.
+  reflexivity.
+Qed.
+
+Program Definition llcons A n (x : A) (xs : llist A n) : llist A (S n) := cons x xs.
+Obligation 1.
+ destruct xs; subst.
+ reflexivity.
+Qed.
+
+Program Definition llnil A : llist A 0 := nil.
+
+Program Definition llhead A n (l : llist A (S n)) : A :=
+  match l with
+  | nil => _
+  | cons x xs => x
+  end.
+Obligation 1.
+ destruct l.
+ simpl in *.
+ subst; inversion e.
+Qed.
+
+Program Definition lltail A n (l : llist A (S n)) : llist A n :=
+  match l with
+  | nil => _
+  | cons x xs => xs
+  end.
+Obligation 1.
+ destruct l; simpl in *; subst.
+ inversion e.
+Qed.
+Obligation 2.
+  revert l x xs Heq_l.
+  induction n; intuition;
+   destruct l; simpl in *; subst;
+   inversion e; reflexivity.
+Qed.
+
+Program Definition llsnoc A n (l : llist A n) a : llist A (S n) :=
+  l ++ (a :: nil).
+Obligation 1.
+ rewrite app_length.
+ rewrite plus_comm.
+ destruct l.
+ subst; reflexivity.
+Qed.
+
+Program Fixpoint llcohead A n (l : llist A (S n)) : A :=
+  match l with
+  | nil => _
+  | cons x xs => match n with
+     | O => x
+     | S m => llcohead (n:=m) xs end
+  end.
+Obligation 1.
+ destruct l; simpl in *; subst.
+ inversion e.
+Qed.
+Obligation 2.
+ destruct l; simpl in *; subst.
+ inversion e; auto.
+Qed.
+
+
+Program Fixpoint llcotail A n (l : llist A (S n)) : llist A n :=
+  match l with
+  | nil => _
+  | cons x xs => match n with
+    | O => nil
+    | S m => cons x (llcotail (n:=m) xs) end
+  end.
+Next Obligation.
+ destruct l; simpl in *; subst.
+ inversion e.
+Qed.
+Next Obligation.
+ destruct l; simpl in *; subst.
+ inversion e; auto.
+Qed.
+
+
+ 
+
+
+  Hint Resolve ll_proj_eq.
+  Lemma llist_head_tail A n (l : llist A (S n)) : llcons (llhead l) (lltail l) = l.
+   destruct l.
+   destruct x.
+    inversion e.
+    auto with *.
+  Defined.
+
+  Hint Resolve llist_head_tail.
+
+  Lemma llist_ind A : forall P : (forall n, llist A n -> Type),
+    P O (llnil A) ->
+    (forall n l, P n l -> forall a, P (S n) (llcons a l)) ->
+    (forall n l, P n l).
+   intros.
+   induction n.
+    destruct l.
+    destruct x; subst.
+     match goal with |- P 0 ?x => replace x with (llnil A); auto end.
+     inversion e.
+   
+    replace l with (llcons (llhead l) (lltail l)); auto.
+  Defined.    
+
+  Lemma llist_ind0 A : forall P : (llist A 0 -> Type),
+    P (llnil A) -> (forall l, P l).
+   intros.
+   destruct l.
+    destruct x; subst.
+     match goal with |- P ?K => replace K with (llnil A); auto end.
+     inversion e.
+  Defined.
+
+  Lemma llist_indS A : forall P : (forall n, llist A (S n) -> Type),
+    (forall a,  P O (llcons a (llnil A))) ->
+    (forall n l, P n l -> forall a, P (S n) (llcons a l)) ->
+    (forall n l, P n l).
+   intros.
+   induction n.
+    destruct l.
+    destruct x; subst.
+     inversion e.
+     match goal with |- P 0 ?x => replace x with (llcons a (llnil A)); auto end.
+     inversion e.
+      destruct x.
+       auto.
+       inversion H0.
+   
+    replace l with (llcons (llhead l) (lltail l)); auto.
+  Defined.
+
+  Lemma llist_cotail A n a (l : llist A (S n)) :
+      llcotail (llcons a l) = llcons a (llcotail l).
+   revert a.
+   revert n l.
+   refine (llist_indS (fun l => _) _ _); intros.
+    auto.
+    rewrite H.
+    apply ll_proj_eq.
+    simpl.
+    repeat f_equal.
+    apply ll_proj_eq; auto.
+  Qed.
+
+  Lemma llist_cohead A n a (l : llist A (S n)) :
+      llcohead (llcons a l) = llcohead l.
+   destruct l.
+   simpl.
+   f_equal.
+   apply ll_proj_eq.
+   reflexivity.
+  Qed.
+
+  Lemma llist_snoc_cons A n a b (l : llist A n) :
+     llsnoc (llcons a l) b = llcons a (llsnoc l b).
+   revert a b.
+   induction l using llist_ind; intros.
+    auto.
+    auto.
+  Qed.
+
+  Lemma llist_cohead_cotail A n (l : llist A (S n)) :
+     llsnoc (llcotail l) (llcohead l) = l.
+   revert n l;
+   refine (llist_indS (fun l => _) _ _); intros.
+    auto.
+    rewrite llist_cotail.
+    rewrite llist_snoc_cons.
+    f_equal.
+    auto.
+    rewrite llist_cohead.
+    trivial.
+  Qed.
+
+Lemma llist_snoc_ind A : forall P : (forall n, llist A n -> Type),
+    P O (llnil A) ->
+    (forall n l, P n l -> forall a, P (S n) (llsnoc l a)) ->
+    (forall n l, P n l).
+ intros.
+ induction n.
+  destruct l.
+  destruct x; subst.
+   match goal with |- P 0 ?x => replace x with (llnil A); auto end.
+   inversion e.
+
+  rewrite <- llist_cohead_cotail.
+  firstorder.
+Qed.
+
+
+Ltac llniltac := 
+ match goal with L : llist _ 0 |- _ => revert L; refine (llist_ind0 (fun L => _) _) end.
+
+
+
+Lemma ll_snoc_rev_cons A n (l : llist A n) a : llcons a (llrev l) = llrev (llsnoc l a).
+ revert a.
+ induction l using llist_ind.
+  auto.
+
+  intros.
+
+  apply ll_proj_eq.
+  simpl.
+  rewrite app_comm_cons.
+  f_equal.
+  generalize (IHl a0); intro.
+  inversion H.
+  firstorder.
+Qed.
+ 
+
+  Lemma llist_tail_cons A n a (l : llist A n) : lltail (llcons a l) = l.
+   auto.
+  Qed.
+
+
+Lemma ll_cons_rev_snoc : forall A n (l : llist A n) a, llrev (llcons a l) = llsnoc (llrev l) a.
+ auto.
+Qed.
+
+Lemma llist_ind1 A : forall P : (llist A 1 -> Type),
+    (forall a, P (llcons a (llnil A))) -> (forall l, P l).
+ intros.
+ rewrite <- (llist_head_tail).
+ generalize (lltail l); intro;
+  llniltac.
+ auto.
+Defined.
+Lemma llist_head_cons A n a (l : llist A n) : llhead (llcons a l) = a.
+reflexivity.
+Qed.
+
+Lemma llist_cohead_snoc A n a (l : llist A n) : llcohead (llsnoc l a) = a.
+induction l using llist_ind.
+auto.
+rewrite llist_snoc_cons.
+rewrite <- IHl at 2.
+rewrite llist_cohead.
+auto.
+Qed.
+
+Lemma llhead_cohead A n (l : llist A (S n)) : llhead (llrev l) = llcohead l.
+  rewrite <- (llist_cohead_cotail l).
+  rewrite <- ll_snoc_rev_cons.
+  rewrite llist_head_cons.
+  rewrite llist_cohead_snoc.
+  auto.
+Qed.
+
+Lemma llist_tail_snoc A n a (l : llist A (S n)) : lltail (llsnoc l a) = llsnoc (lltail l) a.
+  revert n l; apply llist_indS; intros;
+  auto.
+Qed.
+
+Hint Resolve llist_cotail.
+Lemma ll_tail_rev_cotail A n (l : llist A (S n)) : lltail (llrev l) = llrev (llcotail l).
+  revert n l; apply llist_indS; intros.
+  auto.
+  rewrite ll_cons_rev_snoc.
+  rewrite llist_tail_snoc.
+  rewrite H.
+  rewrite <- ll_cons_rev_snoc.
+  f_equal; auto.
+Qed.
+Hint Resolve ll_tail_rev_cotail.
+
